messageInvariantPrototypes/twoPhaseCommit/decentralizedMonotonic/messageInvariants.dfy
@@ -1,0 +1,191 @@
+// Network-level "boilerplate" invariants that are application-independent
+
+include "spec.dfy"
+
+module MessageInvariants {
+import opened Types
+import opened UtilitiesLibrary
+import opened DistributedSystem
+import opened Obligations
+
+// All VoteMsg have a valid participant HostId as src
+ghost predicate VoteMsgValidSrc(c: Constants, v: Variables)
+  requires v.WF(c)
+{
+  forall msg | msg in v.network.sentMsgs && msg.VoteMsg? 
+  :: c.ValidParticipantId( msg.src)
+}
+
+// Every VoteMsg is received according to CoordinatorHost.NextReceiveStepRecvFunc
+ghost predicate RecvVoteMsgValidity(c: Constants, v: Variables) 
+  requires v.WF(c)
+  requires ValidHistory(c, v)
+{
+  reveal_ValidHistory();
+  forall i, idx, msg | 
+    && 1 <= i < |v.history|
+    && c.ValidCoordinatorId(idx)
+    && IsReceiveStepByActor(c, v, i, idx, msg)
+    && msg.VoteReqMsg?
+  :: 
+    && msg in v.network.sentMsgs
+    && CoordinatorHost.NextReceiveStepRecvFunc(c.hosts[idx].coordinator, v.History(i-1).hosts[idx].coordinator, v.History(i).hosts[idx].coordinator, msg)
+}
+
+// Every DecideMsg is sent according to a CoordinatorHost.NextDecisionStepSendFunc
+ghost predicate SendDecideMsgValidity(c: Constants, v: Variables)
+  requires v.WF(c)
+  requires VoteMsgValidSrc(c, v)
+{
+  forall msg | 
+    && msg in v.network.sentMsgs
+    && msg.DecideMsg?
+  :: 
+  (exists i ::
+      && v.ValidHistoryIdx(i)
+      && CoordinatorHost.NextDecisionStepSendFunc(c.GetCoordinator(), v.History(i).GetCoordinator(c), msg)
+  )
+}
+
+// Every VoteReqMsg is received according to ParticipantHost.NextReceiveVoteReqStepRecvFunc
+ghost predicate RecvVoteReqMsgValidity(c: Constants, v: Variables) 
+  requires v.WF(c)
+  requires ValidHistory(c, v)
+{
+  reveal_ValidHistory();
+  forall i, idx, msg | 
+    && 1 <= i < |v.history|
+    && c.ValidParticipantId(idx)
+    && IsReceiveStepByActor(c, v, i, idx, msg)
+    && msg.VoteReqMsg?
+  :: 
+    && msg in v.network.sentMsgs
+    && ParticipantHost.NextReceiveVoteReqStepRecvFunc(c.hosts[idx].participant, v.History(i-1).hosts[idx].participant, v.History(i).hosts[idx].participant, msg)
+}
+
+// Every DecideMsg is received according to ParticipantHost.NextReceiveDecisionStepRecvFunc
+ghost predicate RecvDecideMsgValidity(c: Constants, v: Variables) 
+  requires v.WF(c)
+  requires ValidHistory(c, v)
+{
+  reveal_ValidHistory();
+  forall i, idx, msg | 
+    && 1 <= i < |v.history|
+    && c.ValidParticipantId(idx)
+    && IsReceiveStepByActor(c, v, i, idx, msg)
+    && msg.DecideMsg?
+  :: 
+    && msg in v.network.sentMsgs
+    && ParticipantHost.NextReceiveDecisionStepRecvFunc(c.hosts[idx].participant, v.History(i-1).hosts[idx].participant, v.History(i).hosts[idx].participant, msg)
+}
+
+// Every VoteMsg is sent according to ParticipantHost.NextSendVoteStepSendFunc
+ghost predicate SendVoteMsgValidity(c: Constants, v: Variables)
+  requires v.WF(c)
+  requires VoteMsgValidSrc(c, v)
+{
+  forall msg | 
+    && msg in v.network.sentMsgs
+    && msg.VoteMsg?
+  :: 
+  (exists i ::
+      && v.ValidHistoryIdx(i)
+      && ParticipantHost.NextSendVoteStepSendFunc(c.hosts[msg.src].participant, v.History(i).hosts[msg.src].participant, msg)
+  )
+}
+
+
+ghost predicate MessageInv(c: Constants, v: Variables)
+{
+  && v.WF(c)
+  && ValidHistory(c, v)
+  && VoteMsgValidSrc(c, v)
+  && RecvVoteMsgValidity(c, v)
+  && SendDecideMsgValidity(c, v)
+  && RecvVoteReqMsgValidity(c, v)
+  && RecvDecideMsgValidity(c, v)
+  && SendVoteMsgValidity(c, v)
+}
+
+lemma InitImpliesMessageInv(c: Constants, v: Variables)
+  requires Init(c, v)
+  ensures MessageInv(c, v)
+{
+  InitImpliesValidHistory(c, v);
+}
+
+lemma MessageInvInductive(c: Constants, v: Variables, v': Variables)
+  requires MessageInv(c, v)
+  requires Next(c, v, v')
+  ensures MessageInv(c, v')
+{
+  InvNextValidHistory(c, v, v');
+  InvNextRecvVoteMsgValidity(c, v, v');
+  InvNextSendDecideMsgValidity(c, v, v');
+  InvNextRecvVoteReqMsgValidity(c, v, v');
+  InvNextRecvDecideMsgValidity(c, v, v');
+}
+
+/***************************************************************************************
+*                                         Proofs                                       *
+***************************************************************************************/
+
+lemma InvNextRecvVoteMsgValidity(c: Constants, v: Variables, v': Variables)
+  requires v.WF(c) && v'.WF(c)
+  requires ValidHistory(c, v) && ValidHistory(c, v')
+  requires RecvVoteMsgValidity(c, v)
+  requires Next(c, v, v')
+  ensures RecvVoteMsgValidity(c, v')
+{
+  reveal_ValidHistory();
+  VariableNextProperties(c, v, v');
+}
+
+lemma InvNextRecvVoteReqMsgValidity(c: Constants, v: Variables, v': Variables)
+  requires v.WF(c) && v'.WF(c)
+  requires ValidHistory(c, v) && ValidHistory(c, v')
+  requires RecvVoteReqMsgValidity(c, v)
+  requires Next(c, v, v')
+  ensures RecvVoteReqMsgValidity(c, v')
+{
+  reveal_ValidHistory();
+  VariableNextProperties(c, v, v');
+}
+
+lemma InvNextSendDecideMsgValidity(c: Constants, v: Variables, v': Variables)
+  requires v.WF(c) && v'.WF(c)
+  requires ValidHistory(c, v) && ValidHistory(c, v')
+  requires VoteMsgValidSrc(c, v)
+  requires SendDecideMsgValidity(c, v)
+  requires Next(c, v, v')
+  ensures SendDecideMsgValidity(c, v')
+{
+  reveal_ValidHistory();
+  VariableNextProperties(c, v, v');
+}
+
+lemma InvNextRecvDecideMsgValidity(c: Constants, v: Variables, v': Variables)
+  requires v.WF(c) && v'.WF(c)
+  requires ValidHistory(c, v) && ValidHistory(c, v')
+  requires RecvDecideMsgValidity(c, v)
+  requires Next(c, v, v')
+  ensures RecvDecideMsgValidity(c, v')
+{
+  reveal_ValidHistory();
+  VariableNextProperties(c, v, v');
+}
+
+lemma InvNextSendVoteMsgValidity(c: Constants, v: Variables, v': Variables)
+  requires v.WF(c) && v'.WF(c)
+  requires ValidHistory(c, v) && ValidHistory(c, v')
+  requires VoteMsgValidSrc(c, v)
+  requires SendVoteMsgValidity(c, v)
+  requires Next(c, v, v')
+  ensures SendVoteMsgValidity(c, v')
+{
+  reveal_ValidHistory();
+  VariableNextProperties(c, v, v');
+}
+
+}
+
